compiler/pollang/ReflexKStateDisable.v
@@ -10,16 +10,16 @@ Definition NB_MSG : nat := 2.
 
 Definition PAY_DESC : vvdesc NB_MSG :=
   ( existT _ 1 (str_d, tt) (*User name payload.*)
-   , ( existT _ 2 (str_d, (num_d, tt)) (*Auth response from system payload.*)
+   , ( existT _ 1 (str_d, tt) (*Successful auth response from system payload.*)
     , tt)
   ).
 
 Definition INIT_ENVD : vdesc := existT _ 0 tt.
 
-Definition KST_DESC_SIZE := 2.
+Definition KST_DESC_SIZE := 1.
 
 (*State is (username, authres)*)
-Definition KST_DESC : vdesc' KST_DESC_SIZE := (str_d, (num_d, tt)).
+Definition KST_DESC : vdesc' KST_DESC_SIZE := (num_d, tt).
 
 Definition INIT : @init_prog NB_MSG PAY_DESC _ KST_DESC INIT_ENVD :=
   nil.
@@ -30,34 +30,25 @@ Definition HANDLERS : handlers (VVD := PAY_DESC) KST_DESC :=
       @sdenote _ SDenoted_vdesc (lkup_tag (VVD := PAY_DESC) _tm) -> _
     with
     | None => fun pl =>
-       let (u, _) := pl in
+       let (s, _) := pl in
        let envd := existT _ 0 tt in
        if num_eq (@shvec_ith _ _ _
                                 (KST_DESC:svec desc KST_DESC_SIZE)
-                                (kst _ st) (Some None))
-                    (num_of_nat 0)
-       then existT _ envd (nil) (*Ignore.*)
-       else if str_eq (@shvec_ith _ _ _
-                                (KST_DESC:svec desc KST_DESC_SIZE)
                                 (kst _ st) None)
-                    u
-            then existT _ envd (
+                    (num_of_nat 0)
+       then existT _ envd (
                           let (u, _) := pl in
                           Send _ _ _
                                (HEchan _ _)
                                (@MEmsg _ PAY_DESC envd None (SLit _ u, tt))
                                :: nil
                           )
-            else existT _ envd (nil) (*Ignore.*)
-    | Some None => fun pl =>
+       else existT _ envd (nil) (*Ignore.*)
+    | Some None => fun _ =>
        let envd := existT _ 0 tt in
        existT _ envd (
-        let (u, pl') := pl in
-        let (res, _) := pl' in
         STChange KST_DESC _ _
-          None (HEexpr _ _ _ (MEbase _ _ (SLit _ u)))
-        :: STChange KST_DESC _ _
-             (Some None) (HEexpr _ _ _ (MEbase _ _ (NLit _ res)))
+             None (HEexpr _ _ _ (MEbase _ _ (NLit _ (num_of_nat 1))))
         :: nil
       )
     | Some (Some bad) => fun _ =>
@@ -65,21 +56,21 @@ Definition HANDLERS : handlers (VVD := PAY_DESC) KST_DESC :=
     end (pay m)
   ).
 
+Require Import Ynot.
 Require Import PolLang.
 Require Import ActionMatch.
 Require Import Tactics.
-Require Import Ynot.
 
-Theorem release : forall st tr u,
+Theorem disable : forall st tr,
   Reach _ _ INIT HANDLERS st -> ktr _ st = inhabits tr ->
-  Release NB_MSG PAY_DESC
-          (@KORecv NB_MSG PAY_DESC None
-                   (Some (@Build_opt_msg NB_MSG PAY_DESC
-                                         (Some None) (Some u, (None, tt)))))
-          (@KOSend NB_MSG PAY_DESC None
-                   (Some (@Build_opt_msg NB_MSG PAY_DESC
-                                         None (Some u, tt))))
-          tr.
+  Disables NB_MSG PAY_DESC
+           (@KORecv NB_MSG PAY_DESC None
+                    (Some (@Build_opt_msg NB_MSG PAY_DESC
+                                          (Some None) (None, tt))))
+           (@KOSend NB_MSG PAY_DESC None
+                    (Some (@Build_opt_msg NB_MSG PAY_DESC
+                                          None (None, tt))))
+           tr.
 Proof.
   crush.
 Qed.
