compiler/pollang/Tactics.v
@@ -3,35 +3,129 @@ Require Import PolLang.
 Require Import Reflex.
 Require Import ReflexDenoted.
 Require Import ReflexFin.
+Require Import ReflexBase.
 Require Import Ynot.
+Require Import List.
 
-Ltac unpack :=
-  match goal with
-  | [ s : kstate _, H : ?s = _,
-      s' : kstate _, H' : ?s' = kstate_run_prog ?KST_DESC _ _ _ ?s _ |- _ ]
-      => rewrite H in H'; apply f_equal with (f:=ktr KST_DESC) in H';
-         simpl in H'; rewrite H' in *; unpack
-  | [ s : init_state _ _, H : ?s = _ |- _ ]
-      (*This is problematic because it destroys information about s*)
-      => rewrite H in *; simpl in *; unpack
-  | [ H: [_]%inhabited = [_]%inhabited |- _ ]
-      => apply pack_injective in H;
-         rewrite -> H in * || rewrite <- H in *
+(********Begin General Tactics*********)
+
+Ltac destruct_fin f :=
+  match type of f with
+  | False => destruct f
+  | _ => let f' := fresh "f" in
+         destruct f as [ f' | ]; [destruct_fin f' | ]
+  end.
+
+Ltac destruct_pay pay :=
+  match type of pay with
+  | unit => idtac
+  | _ => let a := fresh "a" in
+         let b := fresh "b" in
+         destruct pay as [a b]; simpl in a; destruct_pay b
   end.
 
 Ltac destruct_msg :=
   match goal with
-  (*Tag is Some False*)
-  | [ f : False |- _ ]
-      => destruct f
-  | [ f : option _, pay : s[[lkup_tag (Some ?f)]] |- _ ]
-      => destruct f; destruct_msg
-  | [ pay : s[[lkup_tag _]] |- _ ]
-      => destruct pay; simpl in *
-  | [ tag : fin _ |- _ ]
-      => destruct tag; destruct_msg
   | [ m : msg |- _ ]
-      => destruct m; destruct_msg
+      => destruct m as [tag pay]; destruct_fin tag;
+         destruct_pay pay
+  end.
+
+(*Destructs num, str, or fd equalities in the context.*)
+Ltac destruct_eq hdlrs H :=
+  unfold hdlrs in H; simpl in H;
+  match type of H with
+  | context[num_eq ?a ?b]
+    => destruct (num_eq a b); simpl in *; destruct_eq hdlrs H
+  | context[str_eq ?a ?b]
+    => destruct (str_eq a b); simpl in *; destruct_eq hdlrs H
+  | context[fd_eq ?a ?b]
+    => destruct (fd_eq a b); simpl in *; destruct_eq hdlrs H
+  | _
+    => idtac
+  end.
+
+Ltac unpack :=
+  match goal with
+  | [ H : ?s = _, H' : ?s' = kstate_run_prog ?KST_DESC _ _ _ ?s _ |- _ ]
+      => rewrite H in H'; rewrite H' in *; simpl in *; unpack
+  | [ s : init_state _ _ |- _ ]
+      => match goal with
+         | [ H : s = _ |- _ ]
+             => rewrite H in *; simpl in *; unpack
+         end
+  | [ tr : KTrace |- _ ]
+      => match goal with
+         | [ H: [_]%inhabited = [tr]%inhabited |- _ ]
+             => apply pack_injective in H; subst tr
+         | [ H: [tr]%inhabited = [_]%inhabited |- _ ]
+             => apply pack_injective in H; subst tr
+         end
+  end.
+
+(*Erases hypothesis relating to old states on which we are not performing induction.*)
+(*First rewrites those states to avoid losing information.*)
+Ltac clear_old_hyps :=
+  match goal with
+  | [ s : kstate _, s' : kstate _ |- _ ]
+      => match goal with
+         | [ H : s = _, H' : s' = _,
+             IHReach : forall tr : KTrace, _ |- _ ]
+           => subst s; subst s'; clear IHReach
+         end
+  end.
+
+Ltac destruct_unpack :=
+  match goal with
+  | [ m : msg, H : _ = kstate_run_prog _ _ _ _ _ _,
+      H' : Reach _ _ _ ?HDLRS _ |- _ ]
+      => destruct_msg; destruct_eq HDLRS H; unpack
+  | [ m : msg |- _ ]
+      => destruct_msg; unpack
+  | _
+      => unpack
+  end.
+
+Ltac subst_states :=
+  match goal with 
+  | [ s : kstate _ |- _ ]
+      => match goal with
+         | [ _ : s = _ |- _ ]
+             => subst s; subst_states
+         end
+  | _
+      => idtac
+  end.
+
+Ltac subst_assignments :=
+  match goal with
+  | [ a := _ |- _ ]
+      => subst a; subst_assignments
+  | _
+      => idtac
+  end.
+
+Ltac destruct_conjuncts H :=
+  match type of H with
+  | _ /\ _ => let L := fresh "L" in
+              let R := fresh "R" in
+              destruct H as [L R]; destruct_conjuncts R
+  | _ => idtac
+  end.
+
+Ltac destruct_disjuncts H :=
+  match type of H with
+  | _ \/ _ => let L := fresh "L" in
+              let R := fresh "R" in
+              destruct H as [L | R]; destruct_disjuncts R
+  | _ => idtac
+  end.
+
+Ltac destruct_action_match :=
+  match goal with
+  | [ H : AMatch ?future ?act |- _ ]
+      => compute in H (*produces a conjunction of Props*);
+         destruct_conjuncts H
   end.
 
 Ltac act_match :=
@@ -42,28 +136,6 @@ Ltac act_match :=
          destruct H; [ assumption | contradiction ]
   end.
 
-Ltac match_immbefore := 
-  match goal with
-  | [ |- ImmBefore _ _ _ _ nil ]
-      => constructor
-  (*Induction hypothesis*)
-  | [ H : ktr _ ?s = inhabits ?tr,
-      IH : forall tr', inhabits tr' = ktr _ ?s ->
-                       ImmBefore _ _ ?oact_b ?oact_a tr'
-                       |- ImmBefore _ _ ?oact_b ?oact_a ?tr ]
-      => auto
-  | [ H : AMatch ?oact_a ?act |- ImmBefore _ _ _ ?oact_a (?act::_::_) ]
-      => apply IB_A; [ match_immbefore | act_match ]
-  | [ H : AMatch ?oact_a ?act |- ImmBefore _ _ _ ?oact_a (?act::_) ]
-      => contradiction
-  | [ H : ~ AMatch ?oact_a ?act |- ImmBefore _ _ _ ?oact_a (?act::_) ]
-      => apply IB_nA; [ match_immbefore | assumption ]
-  | [ |- ImmBefore ?nb_msg ?pdv _ ?oact_a (?act::_) ]
-     => let H := fresh "H" in
-        pose proof (decide_act nb_msg pdv oact_a act) as H;
-        destruct H; match_immbefore
-  end.
-
 Ltac act_nmatch :=
   match goal with
   | [ |- ~@AMatch ?nb_msg ?pdv ?oact ?act ]
@@ -72,43 +144,232 @@ Ltac act_nmatch :=
          destruct H; [ contradiction | assumption ]
   end.
 
-Ltac match_immafter := 
-  match goal with
-  | [ |- ImmAfter _ _ _ _ nil ]
-      => constructor
-  | [ H : ktr _ ?s = inhabits ?tr,
-      IH : forall tr', inhabits tr' = ktr _ ?s ->
-                       ImmAfter _ _ ?oact_a ?oact_b tr'
-                       |- ImmAfter _ _ ?oact_a ?oact_b ?tr ]
-      => auto
-  | [ H : AMatch ?oact_b ?act |- ImmAfter ?nb_msg ?pdv _ ?oact_b (_::?act::_) ]
-      => apply IA_B; [ match_immafter | act_match ] || idtac
-  | [ H : ~AMatch ?oact_b ?act |- ImmAfter ?nb_msg ?pdv _ ?oact_b (_::?act::_) ]
-      => apply IA_nB; [ match_immafter | act_nmatch ] || idtac
-  | [ |- ImmAfter ?nb_msg ?pdv _ ?oact_b (_::?act::_) ]
-      => let H := fresh "H" in
-         pose proof (decide_act nb_msg pdv oact_b act) as H;
-         destruct H; match_immafter
-  | [ |- ImmAfter _ _ _ _ (?act::_) ]
-      => apply IA_nB; [ match_immafter | act_nmatch ]
-  end.
-
 Ltac msg_fds_are_ok :=
   match goal with
   | [ H : ~msg_fds_ok _ _ _ |- _ ]
       => contradict H; compute; msg_fds_are_ok
   | [ |- forall i : _, _ ]
-      => intro i; destruct i; contradiction || auto
+      => intro i; destruct_fin i; contradiction || auto
   end.
 
-Ltac crush :=
+Ltac reach_induction :=
+  intros;
   match goal with
-  | [ m : msg |- _ ]
-      => destruct_msg; crush
+  | [ _ : ktr _ _ = inhabits ?tr, H : Reach _ _ _ _ _ |- _ ]
+      => generalize dependent tr; induction H;
+         simpl in *; intros; destruct_unpack;
+         try msg_fds_are_ok
+         (*msg_fds_are_ok eliminates bad fds case when that's impossible.*)
+  end.
+
+(********End General Tactics*********)
+
+(********Begin Disable Tactics*********)
+
+Ltac use_IH_disables :=
+  match goal with
+  | [ IHReach : ?H -> ?rest, H' : ?H, _ : ktr _ ?s = inhabits ?tr |- _ ]
+    => match rest with
+       | context[forall tr' : KTrace, ktr _ s = inhabits tr' -> _]
+          => let act := fresh "act" in
+             let H'' := fresh "H" in
+             apply IHReach with (tr':=tr) in H'; auto
+             (*TODO: What if there is more than one hypothesis?*)
+       end
+  end.
+
+Ltac forall_not_disabler :=
+  let HIn := fresh "HIn" in
+  let act' := fresh "act'" in
+  (*Checks the concrete actions at the head of the trace.*)
+  intros act' HIn; simpl in HIn; destruct_disjuncts HIn;
+  try (subst act'; simpl; tauto);
+  destruct_action_match;
+  clear_old_hyps;
+  reach_induction;
+  match goal with
+  | [ H : _ = initial_init_state _ _, H' : context[ In _ _ ] |- _ ]
+      => destruct_disjuncts H'; (subst act'; tauto) || contradiction
+         (*subst act' works when it is set equal to actual action*)
+         (*contradiction works when act' is in nil*)
+  | [ H' : context[ In _ _ ] |- _ ]
+      => subst_assignments; subst_states; simpl in *;
+         destruct_disjuncts H';
+         (subst act'; tauto) || discriminate || use_IH_disables
+  end.
+
+Ltac match_disables :=
+  match goal with
+  | [ |- Disables _ _ _ _ nil ]
+      => constructor
+  (* Induction hypothesis.*)
+  | [ H : ktr _ ?s = inhabits ?tr,
+      IH : forall tr', ktr _ ?s = inhabits tr' ->
+                       Disables _ _ ?past ?future tr'
+                       |- Disables _ _ ?past ?future ?tr ]
+      => auto
+  (*Branch on whether the head of the trace matches.*)
+  | [ |- Disables ?nb_msg ?pdv _ ?future (?act::_) ]
+      => let H := fresh "H" in
+         pose proof (decide_act nb_msg pdv future act) as H;
+         destruct H;
+         [ contradiction ||
+           (apply D_disablee; [ match_disables | forall_not_disabler ])
+         | contradiction ||
+           (apply D_not_disablee; [ match_disables | assumption ]) ]
+         (*In some cases, one branch is impossible, so contradiction
+           solves the goal immediately.
+           In other cases, there are variables in the message payloads,
+           so both branches are possible.*)
+  end.
+
+(********End Disable Tactics********)
+
+(********Begin Releases Tactics********)
+
+(*Should only be called by releaser_match.*)
+Ltac releaser_match' :=
+  match goal with
+  | [ |- (?act = _ \/ ?disj_R ) /\ ?conj_R ]
+    => (instantiate (1:=act); compute; tauto) ||
+       (cut (disj_R /\ conj_R); [ | releaser_match']; tauto)
+       (*The last call to tauto solves the first goal created by cut.
+         However, it can't solve this goal until the existential variable
+         is instantiated, which happens in the recursive call to releaser_match'.*)
+  | _ => fail 1
+  end.
+
+Ltac releaser_match :=
+  eexists; releaser_match'.
+
+Ltac use_IH_releases :=
+  match goal with
+  | [ IHReach : ?H -> ?rest, H' : ?H, _ : ktr _ ?s = inhabits ?tr |- _ ]
+    => match rest with
+       | context[forall tr' : KTrace, ktr _ s = inhabits tr' -> _]
+          => let act := fresh "act" in
+             let H'' := fresh "H" in
+             apply IHReach with (tr':=tr) in H'; auto;
+             (*TODO: What if there is more than one hypothesis?*)
+             destruct H' as [ act H'' ]; exists act; tauto
+       end
+  end.
+
+(*TODO: Do we check the actions at the head of the trace? Maybe...*)
+Ltac exists_past :=
+  destruct_action_match;
+  clear_old_hyps;
+  reach_induction;
+  match goal with
+  | [ H : _ = initial_init_state _ _ |- _ ]
+      => rewrite H in *; intuition (*Initial state. Contradiction?*)
+         (*TODO: There may be the action we are looking for in this state.*)
+  | _
+      => subst_assignments; subst_states; repeat subst
+         (*For any equalities generated by destructing the action match*);
+         simpl in *;
+         (contradiction || use_IH_releases || releaser_match)
+         (*destruct_eq might have created contradictions
+           with previous calls of destruct_eq*)
+  end.
+
+Ltac match_releases :=
+  match goal with
+  | [ |- Release _ _ _ _ nil ]
+      => constructor
+  (* Induction hypothesis.*)
+  | [ H : ktr _ ?s = inhabits ?tr,
+      IH : forall tr', ktr _ ?s = inhabits tr' ->
+                       Release _ _ ?past ?future tr'
+                       |- Release _ _ ?past ?future ?tr ]
+      => auto
+  (*Branch on whether the head of the trace matches.*)
+  | [ |- Release ?nb_msg ?pdv _ ?future (?act::_) ]
+      => let H := fresh "H" in
+         pose proof (decide_act nb_msg pdv future act) as H;
+         destruct H;
+         [ contradiction ||
+           (apply R_future; [ match_releases | exists_past ])
+         | contradiction ||
+           (apply R_not_future; [ match_releases | assumption ]) ]
+         (*In some cases, one branch is impossible, so contradiction
+           solves the goal immediately.
+           In other cases, there are variables in the message payloads,
+           so both branches are possible.*)
+  end.
+
+(********End Releases Tactics********)
+
+(*******Begin Immediately Before Tactics********)
+
+Ltac match_immbefore := 
+  match goal with
+  | [ |- ImmBefore _ _ _ _ nil ]
+      => constructor
+  (*Induction hypothesis*)
+  | [ H : ktr _ ?s = inhabits ?tr,
+      IH : forall tr', ktr _ ?s = inhabits tr' ->
+                       ImmBefore _ _ ?oact_b ?oact_a tr'
+                       |- ImmBefore _ _ ?oact_b ?oact_a ?tr ]
+      => auto
+  | [ |- ImmBefore ?nb_msg ?pdv _ ?oact_a (?act::_) ]
+     => let H := fresh "H" in
+        pose proof (decide_act nb_msg pdv oact_a act) as H;
+        destruct H;
+        [ contradiction ||
+          (apply IB_A; [ match_immbefore | act_match ])
+        | contradiction ||
+          (apply IB_nA; [ match_immbefore | assumption ]) ]
+         (*In some cases, one branch is impossible, so contradiction
+           solves the goal immediately.
+           In other cases, there are variables in the message payloads,
+           so both branches are possible.*)
+  end.
+
+(*******End Immediately Before Tactics********)
+
+(*******Begin Immediately After Tactics********)
+
+Ltac match_immafter := 
+  match goal with
+  | [ |- ImmAfter _ _ _ _ nil ]
+      => constructor
+  | [ H : ktr _ ?s = inhabits ?tr,
+      IH : forall tr', ktr _ ?s = inhabits tr' ->
+                       ImmAfter _ _ ?oact_a ?oact_b tr'
+                       |- ImmAfter _ _ ?oact_a ?oact_b ?tr ]
+      => auto
+  | [ |- ImmAfter ?nb_msg ?pdv _ ?oact_b (_::?act::_) ]
+      => let H := fresh "H" in
+         pose proof (decide_act nb_msg pdv oact_b act) as H;
+         destruct H;
+         [ contradiction ||
+           (apply IA_B; [ match_immafter | act_match ] )
+         | contradiction ||
+           (apply IA_nB; [ match_immafter | act_nmatch ] ) ]
+         (*In some cases, one branch is impossible, so contradiction
+           solves the goal immediately.
+           In other cases, there are variables in the message payloads,
+           so both branches are possible.*)
+  | [ |- ImmAfter _ _ _ _ (?act::_) ]
+      (*If theres only one concrete action at the head of the trace,
+        it better not a before action because there's nothing after.*)
+      => apply IA_nB; [ match_immafter | act_nmatch ]
+  end.
+
+(*******End Immediately After Tactics********)
+
+(*******Main Tactic******)
+
+Ltac crush :=
+  reach_induction;
+  match goal with
   | [ |- ImmBefore _ _ _ _ _ ]
-      => unpack; solve [match_immbefore]
+     => match_immbefore
   | [ |- ImmAfter _ _ _ _ _ ]
-      => unpack; solve [match_immafter]
-  | [ H : ~ msg_fds_ok _ _ _ |- _ ]
-      => msg_fds_are_ok
+     => match_immafter
+  | [ |- Disables _ _ _ _ _ ]
+     => match_disables
+  | [ |- Release _ _ _ _ _ ]
+     => match_releases
   end.
